$$
\begin{split}
H|0\rangle &= \frac{1}{\sqrt{2}}(|0\rangle + |1\rangle) = |+\rangle \\
H|0\rangle \oplus H|0\rangle &= |+\rangle \oplus |+\rangle \\
CNOT(|++\rangle) &= |++\rangle \\
H|++\rangle &= |00\rangle \\
\end{split}
$$
---
$$
\begin{split}
H|0\rangle \oplus H|1\rangle &= |+\rangle \oplus |-\rangle \\
CNOT(|+-\rangle) &= |--\rangle \\
H|--\rangle &= |11\rangle \\
\end{split}
$$
---
$$
\begin{split}
H|0\rangle \oplus H|0\rangle &= |+\rangle \oplus |+\rangle \\
CNOT(|++\rangle) &= |++\rangle \\
\end{split}
$$
---
$$
\begin{split}
H|0\rangle \oplus H|1\rangle &= |+\rangle \oplus |-\rangle \\
CNOT(|+-\rangle) &= |--\rangle \\
\end{split}
$$
