$$
u = (2, -7, 1), v = (-3, 0, 4), w = (0, 5, -8) \newline
$$
---
$$
\begin{align}
3u - 4v &= 3(2, -7, 1) - 4(-3, 0, 4) \\
&= (6, -21, 3) - (-12, 0, -16) \\
&= (18, -21, 19)
\end{align}
$$
$$
\begin{align}
2u + 3v - 5w &= 2(2, -7, 1) + 3(-3, 0, 4) - 5(0, 5, -8) \\
&= (4, -14, 2) + (-9, 0, 12) - (0, 25, -40) \\
&= (-5, -39, -26) \\
\end{align}
$$

---

$$
u=\begin{bmatrix}5\\3\\-4\end{bmatrix}, v=\begin{bmatrix}-1\\5\\2\end{bmatrix}, w=\begin{bmatrix}3\\-1\\-2\end{bmatrix}
$$
---
$$
\begin{align}
5u - 2v &= 5\begin{bmatrix}5\\3\\-4\end{bmatrix} - 2\begin{bmatrix}-1\\5\\2\end{bmatrix} \\
&= \begin{bmatrix}25\\15\\-20\end{bmatrix} - \begin{bmatrix}-2\\10\\4\end{bmatrix} \\
5u - 2v &= \begin{bmatrix}27\\5\\-24\end{bmatrix}
\end{align}
$$
$$
\begin{align}
-2u + 4v - 3w &= -2\begin{bmatrix}5\\3\\-4\end{bmatrix} + 4\begin{bmatrix}-1\\5\\2\end{bmatrix} - 3\begin{bmatrix}3\\-1\\-2\end{bmatrix} \\
&= \begin{bmatrix}-10\\-6\\8\end{bmatrix} + \begin{bmatrix}-4\\20\\8\end{bmatrix} - \begin{bmatrix}9\\-3\\-6\end{bmatrix} \\
-2u + 4v - 3w &= \begin{bmatrix}-23\\17\\22\end{bmatrix}
\end{align}
$$
---
Find x and y where
$$
\begin{align}
(a) &, (x,3) = (2, x+y) \\
(b) &, (4,y) = x(2, 3)
\end{align}
$$
---
$$
\begin{align}
(a), (x,3) &= (2, x+y) \\
x &= 2 \\
3 &= x+y = 2 + y \\
y &= 1 \\
(b), (4,y) &= x(2, 3) = (2x, 3x) \\
4 &= 2x \\
x &= 2 \\
y &= 3x = 6
\end{align}
$$
